Let’s solve **Q.1: Solve by Gauss-Jordan Method** step by step.

We are given the system:

```
x -  y + 2z =  3   ---- (1)
x + 2y + 3z =  5   ---- (2)
3x - 4y - 5z = -13 ---- (3)
```

---

### **Step 1: Form the augmented matrix**

\[
\left[
\begin{array}{ccc|c}
1 & -1 & 2 & 3 \\
1 &  2 & 3 & 5 \\
3 & -4 & -5 & -13
\end{array}
\right]
\]

---

### **Step 2: Apply Gauss-Jordan Elimination**

We aim to convert the matrix to **Reduced Row Echelon Form (RREF)**, i.e., the left 3×3 matrix should become the identity matrix.

#### **Step 2.1: Make pivot at (1,1) = 1** (already 1, no change)

\[
R_1 = R_1
\]

#### **Step 2.2: Make all other elements in column 1 = 0**

- \( R_2 = R_2 - R_1 \)
- \( R_3 = R_3 - 3R_1 \)

\[
\left[
\begin{array}{ccc|c}
1 & -1 & 2 & 3 \\
0 & 3  & 1 & 2 \\
0 & -1 & -11 & -22
\end{array}
\right]
\]

---

#### **Step 2.3: Make pivot at (2,2) = 1**

- \( R_2 = \frac{1}{3} R_2 \)

\[
\left[
\begin{array}{ccc|c}
1 & -1 & 2 & 3 \\
0 & 1 & \frac{1}{3} & \frac{2}{3} \\
0 & -1 & -11 & -22
\end{array}
\right]
\]

---

#### **Step 2.4: Make all other elements in column 2 = 0**

- \( R_1 = R_1 + R_2 \)
- \( R_3 = R_3 + R_2 \)

\[
\left[
\begin{array}{ccc|c}
1 & 0 & \frac{7}{3} & \frac{11}{3} \\
0 & 1 & \frac{1}{3} & \frac{2}{3} \\
0 & 0 & -\frac{32}{3} & -\frac{64}{3}
\end{array}
\right]
\]

---

#### **Step 2.5: Make pivot at (3,3) = 1**

- \( R_3 = \left( -\frac{3}{32} \right) R_3 \)

\[
\left[
\begin{array}{ccc|c}
1 & 0 & \frac{7}{3} & \frac{11}{3} \\
0 & 1 & \frac{1}{3} & \frac{2}{3} \\
0 & 0 & 1 & 2
\end{array}
\right]
\]

---

#### **Step 2.6: Make other entries in column 3 = 0**

- \( R_1 = R_1 - \frac{7}{3} R_3 \)
- \( R_2 = R_2 - \frac{1}{3} R_3 \)

\[
\left[
\begin{array}{ccc|c}
1 & 0 & 0 & -1 \\
0 & 1 & 0 & 0 \\
0 & 0 & 1 & 2
\end{array}
\right]
\]

---

### **Final Answer:**

\[
x = -1,\quad y = 0,\quad z = 2
\]

Let me know if you'd like me to move on to Q.2!
